\section{Means and Proofs}
In math there are a lot of means. In this section I will show some of them with the correspoinding proofs.

\begin{itemize}[label=\(-\)]
	\item \textbf{Arithmetic Mean:} The arithmetic mean of \( n \) numbers \( x_1, x_2, \ldots, x_n \) is given by:
	      \[
		      A = \frac{x_1 + x_2 + \ldots + x_n}{n}
	      \]
	\item \textbf{Geometric Mean:} The geometric mean of \( n \) numbers \( x_1, x_2, \ldots, x_n \) is given by:
	      \[
		      G = \sqrt[n]{x_1 \cdot x_2 \cdots x_n}
	      \]
	\item \textbf{Harmonic Mean:} The harmonic mean of \( n \) numbers \( x_1, x_2, \ldots, x_n \) is given by:
	      \[
		      H = \frac{n}{\frac{1}{x_1} + \frac{1}{x_2} + \ldots + \frac{1}{x_n}}
	      \]
	\item \textbf{Quadratic Mean:} The quadratic mean (or root mean square) of \( n \) numbers \( x_1, x_2, \ldots, x_n \) is given by:
	      \[
		      Q = \sqrt{\frac{x_1^2 + x_2^2 + \ldots + x_n^2}{n}}
	      \]
\end{itemize}

\subsection{Proof of the Arithmetic Mean-Geometric Mean Inequality}

Let \( a_1, a_2, \dots, a_n > 0 \). We will prove by induction that:
\[
	\frac{a_1 + a_2 + \cdots + a_n}{n} \geq \sqrt[n]{a_1 a_2 \cdots a_n}
\]
with equality if and only if \( a_1 = a_2 = \cdots = a_n \).

\subsection*{Base Case: \( n = 2 \)}

We want to prove:
\[
	\frac{a_1 + a_2}{2} \geq \sqrt{a_1 a_2}
\]

Let \( a_1, a_2 > 0 \). Then by the identity
\[
	\left( \frac{a_1 - a_2}{2} \right)^2 \geq 0,
\]
we get
\[
	\frac{a_1^2 - 2a_1a_2 + a_2^2}{4} \geq 0 \Rightarrow a_1^2 + a_2^2 \geq 2a_1a_2.
\]
So,
\[
	(a_1 + a_2)^2 \geq 4a_1a_2 \Rightarrow \left( \frac{a_1 + a_2}{2} \right)^2 \geq a_1a_2,
\]
and taking square roots gives the desired result:
\[
	\frac{a_1 + a_2}{2} \geq \sqrt{a_1 a_2}.
\]

\subsection*{For \( n \geq 2 \)}

\[
	A_{n + 1} := (\sum_{i=1}^{n + 1} a_i) / (n + 1) = \frac{a_1 + a_2 + \cdots + a_n + a_{n + 1}}{n + 1}
\]
\[
	G_{n + 1} := \sqrt[n + 1]{a_1 a_2 \cdots a_n a_{n + 1}} = \sqrt[n + 1]{(a_1 a_2 \cdots a_n) a_{n + 1}}
\]
\[
	A_{n - 1}^{n + 1} = (\frac{a_1 + a_2 + \cdots + a_{n + 1}}{n + 1})^{n - 1} = A_{n + 1}^{n - 1}
\]
\[
	G_{n + 1}^{n + 1} := (\sqrt[n + 1]{a_1 a_2 \cdots a_n a_{n + 1}})^{n + 1} = (a_1 a_2 \cdots a_n) a_{n + 1} = \sqrt[n]{(a_1 a_2 \cdots a_n)^{n}} a_{n + 1}^{n + 1} = G_{n}^{n} a_{n + 1}^{n + 1}
\]
Then
\begin{center}
	\(G_{n + 1}^{n + 1}  A_{n + 1}^{n - 1} = G_{n}^{n} a_{n + 1}^{n + 1} A_{n + 1}^{n - 1} \leq A_{n}^{n} A_{n + 1}^{n - 1}\)
\end{center}

This comes from

\begin{center}
	\[
		G_n \leq A_n
	\]
	\[
		G_n^{n} \leq A_n^{n}
	\]
	\[
		G_n^{n} a_{n+1} \leq A_n^{n} a_{n+1}
	\]
	\[
		G_{n}^{n} a_{n + 1}^{n + 1} A_{n + 1}^{n - 1} \leq A_{n}^{n} A_{n + 1}^{n - 1} = \left(A_{n}^{n} \left( a_{n + 1} A_{n +1}\right)^{n -1} \right)^{\frac{n}{n}}
	\]
	\[
		\leq A_{n}^{n} \left( \frac{a_{n + 1} + A_{n + 1} + \dots A_{n + 1}}{n} \right)^{n}
	\]
	\[
		A_{n}^{n} \left( \frac{a_{n + 1} + (n - 1)A_{n + 1}}{n} \right)^{n}
	\]
	\[
		\left( A_{n} \frac{a_{n + 1} + (n - 1)A_{n + 1}}{n} \right)^{n}
	\]
\end{center}

Note that
\begin{center}
	\[
		\left( A_{n} \frac{a_{n + 1} + (n - 1)A_{n + 1}}{n} \right) \rightarrow  \left( \sqrt{A_{n} \frac{a_{n + 1} + (n - 1)A_{n + 1}}{n}} \right)^{2}
	\]
	\[
		\leq \left( \frac{ A_n + \frac{a_{n + 1} + (n - 1)A_{n + 1}}{n}}{2} \right)^{2n}
	\]
\end{center}

Now with power of \textit{n} we have
\begin{center}
	\[
		\left( A_{n} + \frac{a_{n + 1} + (n - 1)A_{n + 1}}{n} \right)^{n} \leq \left( \frac{A_{n} + \frac{a_{n + 1} + (n - 1)A_{n + 1}}{n}}{2} \right)^{2n}
	\]

	\[
		= \left( \frac{A_n}{2} + \frac{a_{n + 1} + (n - 1)A_{n + 1}}{2n}\right)^{2n}
	\]
	\[
		= \left( \frac{A_n n}{2n} + \frac{a_{n + 1} + (n - 1)A_{n + 1}}{2n}\right)^{2n}
	\]
	\[
		= \left( \frac{A_n n  + a_{n + 1} + (n - 1)A_{n + 1}}{2n}\right)^{2n}
	\]
	\[
		= \left( \frac{A_{n + 1}(n + 1) + (n - 1)A_{n + 1}}{2n}\right)^{2n}
	\]
	\[
		= \left( \frac{2n A_{n + 1}}{2n}\right)^{2n} = \left(A_{n + 1}\right)^{2n}
	\]
\end{center}

Now we have prooven that \(G_{n + 1}^{n + 1} A_{n + 1}^{n - 1}\leq \left(A_{n + 1}\right)^{2n}\) by dividing both sides by \( A_{n + 1}^{n - 1} \) we get
\begin{center}
	\[
		G_{n + 1}^{n + 1}\leq A_{n + 1}^{n + 1}
	\]
\end{center}
\QED

\subsection{Proof of the Harmonic Mean Geometric Mean Inequality}
Let \( a_1, a_2, \ldots, a_n > 0 \). We will prove the inequality.
\\
We know that \(G_n \leq A_n \)

\begin{center}
	\[
		G_n \leq A_n
	\]
	\[
		\sqrt[n]{x_1 \cdot x_2 \cdots x_n} \leq \frac{x_1 + x_2 + \ldots + x_n}{n}
	\]
	\[
		\frac{n}{\frac{1}{x_1} + \frac{1}{x_2} + \ldots + \frac{1}{x_n}} \leq \sqrt[n]{x_1 \cdot x_2 \cdots x_n}
	\]
\end{center}
This concludes the proof of the harmonic mean-geometric mean inequality.\\
\QED
\newpage